chapter7/Coq/M/Subtyping_inversion.v
@@ -1,5 +1,6 @@
 Require Import Metalib.Metatheory.
 Require Import LibTactics.
+Require Import Lia.
 Require Import syntax_ott
                rules_inf.
 
@@ -252,6 +253,157 @@ Proof.
     inductions H; try solve[inverts* tl]; try solve[inverts* sta];eauto.
 Qed.
 
+
+Lemma disjoint_eqv_r_aux: forall A B C n,  
+ size_dtyp A + size_dtyp B + size_dtyp C < n ->
+ disjoint A B ->
+ sub A C -> sub B C -> sub dt_top C.
+Proof.
+   introv sz Dis S1 S2.
+   gen A B C.
+   induction n; intros;try solve[lia].
+   inverts Dis; auto;
+   try solve[inverts S1 as h1 h2; inverts S2 as h11 h22; auto;
+   forwards: IHn h1 h11; auto;
+   simpl in *;lia;
+   forwards: IHn h2 h22; auto;
+   simpl in *;lia].
+   -
+     destruct C; auto.
+     +
+     forwards hh1: sub_andl S1; auto.
+     inverts hh1 as hh1.
+     forwards: IHn H hh1 S2; auto.
+     simpl in *; lia; auto.
+     forwards: IHn H0 hh1 S2; auto.
+     simpl in *; lia; auto.
+     +
+     forwards hh1: sub_andl S1; auto.
+     inverts hh1 as hh1.
+     forwards: IHn H hh1 S2; auto.
+     simpl in *; lia; auto.
+     forwards: IHn H0 hh1 S2; auto.
+     simpl in *; lia; auto.
+     +
+     forwards hh1: sub_andl S1; auto.
+     inverts hh1 as hh1.
+     forwards: IHn H hh1 S2; auto.
+     simpl in *; lia; auto.
+     forwards: IHn H0 hh1 S2; auto.
+     simpl in *; lia; auto.
+     +
+     forwards hh1: dand_inversion S1; auto.
+     forwards hh2: dand_inversion S2; auto.
+     inverts hh1 as hh1 hh11.
+     inverts hh2 as hh2 hh22.
+     forwards: IHn hh1 hh2; auto.
+     simpl in *; lia; auto.
+     forwards: IHn hh11 hh22; auto.
+     simpl in *; lia; auto.
+     +
+     forwards hh1: sub_andl S1; auto.
+     inverts hh1 as hh1.
+     forwards: IHn H hh1 S2; auto.
+     simpl in *; lia; auto.
+     forwards: IHn H0 hh1 S2; auto.
+     simpl in *; lia; auto.
+   -
+     destruct C; auto.
+     +
+     forwards hh1: sub_andl S2; auto.
+     inverts hh1 as hh1.
+     forwards: IHn H S1 hh1; auto.
+     simpl in *; lia; auto.
+     forwards: IHn H0 S1 hh1; auto.
+     simpl in *; lia; auto.
+     +
+     forwards hh1: sub_andl S2; auto.
+     inverts hh1 as hh1.
+     forwards: IHn H S1 hh1; auto.
+     simpl in *; lia; auto.
+     forwards: IHn H0 S1 hh1; auto.
+     simpl in *; lia; auto.
+     +
+     forwards hh1: sub_andl S2; auto.
+     inverts hh1 as hh1.
+     forwards: IHn H S1 hh1; auto.
+     simpl in *; lia; auto.
+     forwards: IHn H0 S1 hh1; auto.
+     simpl in *; lia; auto.
+     +
+     forwards hh1: dand_inversion S1; auto.
+     forwards hh2: dand_inversion S2; auto.
+     inverts hh1 as hh1 hh11.
+     inverts hh2 as hh2 hh22.
+     forwards: IHn hh1 hh2; auto.
+     simpl in *; lia; auto.
+     forwards: IHn hh11 hh22; auto.
+     simpl in *; lia; auto.
+     +
+     forwards hh1: sub_andl S2; auto.
+     inverts hh1 as hh1.
+     forwards: IHn H S1 hh1; auto.
+     simpl in *; lia; auto.
+     forwards: IHn H0 S1 hh1; auto.
+     simpl in *; lia; auto.
+   -
+     inverts S1 as h1 h2; inverts S2 as h11 h22; auto.
+     forwards: IHn h1 h11; auto.
+     simpl in *;lia.
+     forwards: IHn h2 h22; auto.
+     simpl in *;lia.
+   -
+     inverts S1 as h1 h2; inverts S2 as h11 h22; auto.
+     forwards: IHn h1 h11; auto.
+     simpl in *;lia.
+     forwards: IHn h2 h22; auto.
+     simpl in *;lia.
+   -
+     inverts S1 as h1 h2; inverts S2 as h11 h22; auto.
+     +
+     forwards: IHn h1 h11; auto.
+     simpl in *;lia.
+     forwards: IHn h2 h22; auto.
+     simpl in *;lia.
+     +
+     exfalso; apply H; auto.
+   -
+     inverts S1 as h1 h2; inverts S2 as h11 h22; auto.
+     forwards: IHn h1 h11; auto.
+     simpl in *;lia.
+     forwards: IHn h2 h22; auto.
+     simpl in *;lia.
+   -
+     inverts S1 as h1 h2; inverts S2 as h11 h22; auto.
+     forwards: IHn h1 h11; auto.
+     simpl in *;lia.
+     forwards: IHn h2 h22; auto.
+     simpl in *;lia.
+   -
+     inverts S1 as h1 h2; inverts S2 as h11 h22; auto.
+     forwards: IHn h1 h11; auto.
+     simpl in *;lia.
+     forwards: IHn h2 h22; auto.
+     simpl in *;lia.
+   -
+     inverts S1 as h1 h2; inverts S2 as h11 h22; auto.
+     forwards: IHn h1 h11; auto.
+     simpl in *;lia.
+     forwards: IHn h2 h22; auto.
+     simpl in *;lia.
+Qed.
+
+
+Lemma disjoint_eqv_r: forall A B,  
+ disjoint A B ->
+ disjointSpec A B.
+Proof.
+   introv dis.
+   unfold disjointSpec;intros.
+   eapply disjoint_eqv_r_aux; eauto.
+Qed.
+
+
 Lemma disjoint_eqv: forall A B,
     disjointSpec A B <-> disjoint A B.
 Proof.
@@ -324,62 +476,7 @@ Proof.
     + destruct(l == l0); eauto. inverts e.
       forwards*: H (dt_rcd l0 dt_top). inverts H0.
   - 
-    intros H C S1 S2.
-    gen B C.
-    induction* A;
-      intros B H;
-      [ induction* B | inductions B | skip | skip | induction* B  ];
-      intros C S1 S2;
-      try solve [inverts H; inverts* H0].
-    + (* int arr *)
-      induction* C;
-      inverts S1;
-      inverts* S2; try solve[inverts* S].
-    + (* int and *)
-      induction* C;
-      inverts H;
-      inverts* S1;  
-      try solve[forwards*: topLike_super_toplc2 H0];
-      try solve[forwards*: sub_andl S2];
-      try solve[forwards*: dand_inversion S2];
-      try solve[inverts* H0].
-    + (* int rcd *)
-      induction* C;
-        inverts S1;
-        inverts* S2.
-    + (* bot top *)
-      induction* C;
-      inverts S1;
-      inverts* S2; try solve[inverts* S].
-    + (* bot and *)
-      induction* C;
-      inverts H;
-      inverts* S1;  
-      try solve[inverts* S2];
-      try solve[forwards*: dand_inversion S2];
-      try solve[inverts* H0].
-    + (* rcd int *)
-      induction* C;
-        inverts S1;
-        inverts* S2.
-    + (* rcd arr *)
-      induction* C;
-        inverts S1;
-        inverts* S2.
-    + (* arr and *)
-        induction* C;
-        inverts H;
-        inverts* S1;  
-        try solve[forwards*: topLike_super_toplc2 H0];
-        try solve[forwards*: sub_andl S2];
-        try solve[forwards*: dand_inversion S2];
-        try solve[inverts* H0].
-    + (* rcd rcd*)
-      induction* C;
-      inverts H;
-      inverts* S1; 
-      try solve[inverts* H0];
-      try solve[inverts* S2].
+    apply disjoint_eqv_r; eauto.
 Qed. 
 
 
